Break Lib.IntTypes abstraction using Declassify

src/tls/Crypto.AE.fsti
@@ -11,7 +11,8 @@ module HST = FStar.HyperStack.ST
 module EE = EverCrypt.Error
 module G = FStar.Ghost
 module F = Flags
-module Cast = Crypto.Util.IntCast
+
+open Declassify
 
 val encrypt
   (#a: SC.supported_alg)
@@ -21,7 +22,7 @@ val encrypt
   (plain_len: U32.t {U32.v plain_len == B.length plain})
   (cipher: cipher_p a) // cipher == iv ++ cipher ++ tag (see EverCrypt.AEAD.encrypt_st)
 : HST.Stack unit
-  (requires (fun h ->
+  (requires fun h ->
     invariant h s /\
     B.live h plain /\
     B.live h cipher /\
@@ -30,13 +31,18 @@ val encrypt
     B.loc_disjoint (footprint s) (B.loc_buffer cipher) /\
     B.disjoint plain cipher /\
     B.length cipher == B.length plain + iv_length + SC.tag_length a
-  ))
-  (ensures (fun h _ h' ->
+    // This is the only difference wrt Crypto.AEAD.encrypt, because
+    // the IV is sampled randomly 
+    //(F.ideal_iv == true ==> fresh_iv h s (B.as_seq h (B.gsub cipher 0ul iv_len)))
+  )
+  (ensures fun h _ h' ->
       let iv = B.gsub cipher 0ul iv_len in
       let cipher' = B.gsub cipher iv_len (B.len cipher `U32.sub` iv_len) in
       B.modifies (B.loc_union (footprint s) (B.loc_buffer cipher)) h h' /\
       invariant h' s /\
-      (F.ideal_AEAD == false ==> SC.encrypt (state_kv s) (Cast.to_seq_sec8 (B.as_seq h' iv)) Seq.empty (Cast.to_seq_sec8 (B.as_seq h plain)) `Seq.equal` Cast.to_seq_sec8 (B.as_seq h' cipher'))
-  ))
+      (F.ideal_AEAD == false ==> 
+       SC.encrypt (state_kv s) (B.as_seq h' iv) Seq.empty (B.as_seq h plain) `Seq.equal`
+       B.as_seq h' cipher')
+  )
 
 // decrypt is unchanged from Crypto.AEAD.decrypt
