src/tls/Crypto.AEAD.fsti
@@ -11,7 +11,8 @@ module HST = FStar.HyperStack.ST
 module EE = EverCrypt.Error
 module G = FStar.Ghost
 module F = Flags
-module Cast = Crypto.Util.IntCast
+
+open Declassify
 
 type plain_pred = (plain: Seq.seq U8.t) -> Tot Type0
 
@@ -31,8 +32,8 @@ val frame_invariant
   (#a: SC.supported_alg) (#phi: plain_pred) (h: HS.mem) (s: state a phi)
   (l: B.loc) (h' : HS.mem)
 : Lemma
-  (requires (B.modifies l h h' /\ B.loc_disjoint l (footprint s) /\ invariant h s))
-  (ensures (invariant h' s))
+  (requires B.modifies l h h' /\ B.loc_disjoint l (footprint s) /\ invariant h s)
+  (ensures  invariant h' s)
 
 inline_for_extraction
 let iv_len = 12ul
@@ -68,12 +69,12 @@ val frame_fresh_iv
   (l: B.loc)
   (h' : HS.mem)
 : Lemma
-  (requires (
+  (requires 
     invariant h s /\
     B.modifies l h h' /\
     B.loc_disjoint l (footprint s)
-  ))
-  (ensures (fresh_iv h' s iv <==> fresh_iv h s iv))
+  )
+  (ensures fresh_iv h' s iv <==> fresh_iv h s iv)
 
 noextract
 val is_fresh_iv
@@ -82,16 +83,16 @@ val is_fresh_iv
   (s: state a phi) // key
   (iv: B.buffer U8.t)
 : HST.Stack bool
-  (requires (fun h -> 
+  (requires fun h -> 
     Flags.ideal_iv == true /\
     invariant h s /\
     B.live h iv /\
     B.len iv == iv_len
-  ))
-  (ensures (fun h res h' ->
+  )
+  (ensures fun h res h' ->
     B.modifies B.loc_none h h' /\
-    (res == true <==> fresh_iv h s (Cast.to_seq_sec8 (B.as_seq h iv)))
-  ))
+    (res == true <==> fresh_iv h s (B.as_seq h iv))
+  )
 
 val encrypt
   (#a: SC.supported_alg)
@@ -103,7 +104,7 @@ val encrypt
   // FIXME: for now we assume that cipher already contains some iv, but at some point
   // we should have `encrypt` randomly generate it and write it into cipher
 : HST.Stack unit
-  (requires (fun h ->
+  (requires fun h ->
     invariant h s /\
     B.live h plain /\
     B.live h cipher /\
@@ -112,17 +113,19 @@ val encrypt
     B.loc_disjoint (footprint s) (B.loc_buffer cipher) /\
     B.disjoint plain cipher /\
     B.length cipher == B.length plain + iv_length + SC.tag_length a /\
-    (F.ideal_iv == true ==> fresh_iv h s (Cast.to_seq_sec8 (B.as_seq h (B.gsub cipher 0ul iv_len))))
-  ))
-  (ensures (fun h _ h' ->
+    (F.ideal_iv == true ==> fresh_iv h s (B.as_seq h (B.gsub cipher 0ul iv_len)))
+  )
+  (ensures fun h _ h' ->
       // FIXME: currently we assume iv already in cipher,
       // at some point it should be randomly generated here
       let iv = B.gsub cipher 0ul iv_len in
       let cipher' = B.gsub cipher iv_len (B.len cipher `U32.sub` iv_len) in
       B.modifies (B.loc_union (footprint s) (B.loc_buffer cipher')) h h' /\
       invariant h' s /\
-      (F.ideal_AEAD == false ==> SC.encrypt (state_kv s) (Cast.to_seq_sec8 (B.as_seq h iv)) Seq.empty (Cast.to_seq_sec8 (B.as_seq h plain)) `Seq.equal` Cast.to_seq_sec8 (B.as_seq h' cipher'))
-  ))
+      (F.ideal_AEAD == false ==> 
+       SC.encrypt (state_kv s) (B.as_seq h iv) Seq.empty (B.as_seq h plain) `Seq.equal` 
+       B.as_seq h' cipher')
+  )
 
 val decrypt
   (#a: SC.supported_alg)
@@ -132,7 +135,7 @@ val decrypt
   (cipher_len: U32.t { U32.v cipher_len == B.length cipher })
   (plain: plain_p a)
 : HST.Stack EE.error_code
-  (requires (fun h ->
+  (requires fun h ->
     invariant h s /\
     B.live h plain /\
     B.live h cipher /\
@@ -140,8 +143,8 @@ val decrypt
     B.loc_disjoint (footprint s) (B.loc_buffer plain) /\
     B.loc_disjoint (footprint s) (B.loc_buffer cipher) /\
     B.disjoint plain cipher
-  ))
-  (ensures (fun h res h' ->
+  )
+  (ensures fun h res h' ->
     let iv' = B.gsub cipher 0ul iv_len in
     let cipher' = B.gsub cipher iv_len (cipher_len `U32.sub` iv_len) in
     match res with
@@ -150,14 +153,15 @@ val decrypt
       invariant h' s /\ (
         if F.ideal_AEAD
         then phi (B.as_seq h' plain)
-        else SC.decrypt (state_kv s) (Cast.to_seq_sec8 (B.as_seq h iv')) Seq.empty (Cast.to_seq_sec8 (B.as_seq h cipher')) == Some (Cast.to_seq_sec8 (B.as_seq h' plain))
+        else SC.decrypt (state_kv s) (B.as_seq h iv') Seq.empty (B.as_seq h cipher') == Some (B.as_seq h' plain)
       )
     | EE.AuthenticationFailure ->
       B.modifies (B.loc_union (footprint s) (B.loc_buffer plain)) h h' /\
       invariant h' s /\
-      (F.ideal_AEAD == false ==> SC.decrypt (state_kv s) (Cast.to_seq_sec8 (B.as_seq h iv')) Seq.empty (Cast.to_seq_sec8 (B.as_seq h cipher')) == None)
+      (F.ideal_AEAD == false ==> 
+       SC.decrypt (state_kv s) (B.as_seq h iv') Seq.empty (B.as_seq h cipher') == None)
     | _ -> False
-  ))
+  )
 
 val create
   (r: HS.rid)
@@ -165,12 +169,12 @@ val create
   (k: B.buffer U8.t) // contains the key
   (phi: plain_pred)
 : HST.ST (option (state a phi))
-  (requires (fun h ->
+  (requires fun h ->
     HST.is_eternal_region r /\
     B.live h k /\
     B.length k == SC.key_length a
-  ))
-  (ensures (fun h res h' ->
+  )
+  (ensures fun h res h' ->
     B.modifies B.loc_none h h' /\
     begin match res with
     | None -> True // supported_alg is not enough to ensure that EverCrypt.AEAD.create_in will succeed (cf. EverCrypt.AEAD.fst: Vale with bad config)
@@ -178,18 +182,14 @@ val create
       B.fresh_loc (footprint s) h h' /\
       B.loc_includes (B.loc_region_only true r) (footprint s) /\
       invariant h' s /\
-      state_kv s == Cast.to_seq_sec8 (B.as_seq h k)
+      state_kv s == B.as_seq h k
     end
-  ))
+  )
 
 val free
   (#a: SC.supported_alg)
   (#phi: plain_pred)
   (s: state a phi)
 : HST.ST unit
-  (requires (fun h ->
-    invariant h s
-  ))
-  (ensures (fun h _ h' ->
-    B.modifies (footprint s) h h'
-  ))
+  (requires fun h -> invariant h s)
+  (ensures  fun h _ h' -> B.modifies (footprint s) h h')
