src/tls/Crypto.AE.fst
@@ -12,43 +12,32 @@ module HST = FStar.HyperStack.ST
 module EE = EverCrypt.Error
 module G = FStar.Ghost
 module F = Flags
-module Cast = Crypto.Util.IntCast
 module E = EverCrypt
 module ES = EverCrypt.Specs
 module Model = Model.AE
 module MU = Model.Utils
-module Cast = Crypto.Util.IntCast
 
 friend Crypto.AEAD // needed because of the definition of state for model
 
-let encrypt
-  #a #phi s plain plain_len cipher
-= let h0 = HST.get () in
+open Declassify
+
+let encrypt #a #phi s plain plain_len cipher = 
+  let h0 = HST.get () in
   if F.model
   then begin
-    let s : Model.state a (mphi phi) = s in
+    let s : Model.state a phi = s in
     let plain_s = MU.get_buffer plain plain_len in
-    let plain_s_sec = Cast.to_seq_sec8 plain_s in
     let cipher_len = iv_len `U32.add` plain_len `U32.add` tag_len a in
     let h1 = HST.get () in
     Model.frame_invariant h0 s B.loc_none h1;
-    Cast.to_seq_uint8_to_seq_sec8 plain_s;
-    let cipher_s_sec = Model.encrypt s plain_s_sec in
+    let cipher_s = Model.encrypt s plain_s in
     let h2 = HST.get () in
-    Cast.live_to_buf_sec8 cipher h2;
-    MU.put_buffer (Cast.to_buf_sec8 cipher) cipher_len cipher_s_sec;
+    MU.put_buffer cipher cipher_len cipher_s;
     let h3 = HST.get () in
-    Cast.loc_buffer_to_buf_sec8 cipher;
-    Cast.to_seq_sec8_as_seq_gsub h3 cipher 0ul iv_len;
-    Cast.to_seq_sec8_as_seq_gsub h3 cipher iv_len (B.len cipher `U32.sub` iv_len);
-    Model.frame_invariant h2 s (B.loc_buffer cipher) h3;
-    ()
+    Model.frame_invariant h2 s (B.loc_buffer cipher) h3
   end else begin
     let iv = B.sub cipher 0ul iv_len in
-    let h1 = HST.get () in
-    Cast.live_to_buf_sec8 iv h1;
-    Random.sample_secret_buffer iv_len (Cast.to_buf_sec8 iv);
-    Cast.loc_buffer_to_buf_sec8 iv;
+    Random.sample_secret_buffer iv_len iv;
     let h2 = HST.get () in
     frame_invariant h0 s (B.loc_buffer cipher) h2;
     encrypt s plain plain_len cipher
